\section{Space-point variance}
\label{App:SciFiSpcPntSD}

Figure \ref{Fig:SenseArea} shows the arrangement of the fibre channels in
the tracker.
The regions in which a space point will be reconstructed are shown by
the shaded areas.
The area of the triangular intersection is given by:
\begin{eqnarray}
  A & = & 4 \frac{1}{2} \frac{c_p}{\sqrt{3}} \frac{c_p}{2} \\
    & = & \frac{c_p^{2}}{\sqrt{3}} \, ;
\end{eqnarray}
where $c_p$ is the channel pitch.
Therefore, for the triangular intersection, the mean values of $x$ and
$y$ are given by:
\begin{eqnarray}
  \bar{x} & = & \frac{1}{A} \int \int x dx dy                           \\
          & = & \frac{1}{A} \int_{0}^{c_p} x dx                         
                \int_{-\frac{x}{\sqrt{3}}}^{\frac{x}{\sqrt{3}}} dy                \\
          & = & \frac{1}{A} \frac{2}{\sqrt{3}} \int_{0}^{c_p} x^{2} dx   \\
          & = & \frac{1}{A} \frac{2}{\sqrt{3}} \frac{c_p^{3}}{3}        \\
          & = & \frac{\sqrt{3}}{c_p^2} \frac{2}{\sqrt{3}} \frac{c_p^{3}}{3}  \\
          & = & \frac{2}{3}c_p \, {\rm ; and}
\end{eqnarray}
\begin{eqnarray}
  \bar{y}&=&\frac{1}{A} \int \int y dx dy                            \\
         &=&\frac{1}{A} \int_{0}^{c_p} dx                            
            \int_{-\frac{x}{\sqrt{3}}}^{\frac{x}{\sqrt{3}}} y dy               \\
         &=&\frac{1}{A}  \int_{0}^{c_p} 
            \left[ \frac{y^{2}}{2} \right]_{-\frac{x}{\sqrt{3}}}^{\frac{x}{\sqrt{3}}} dx \\
         &=&0 \, .
\end{eqnarray}
The variance of the $x$ and $y$ coodinates are then given by:
\begin{eqnarray}
  V_x = \sigma^2_x &=& \frac{1}{A} \int \int (x-\bar{x})^{2} dx dy   \\
                  &=& \frac{1}{A} \int_{0}^{c_p} dx 
                      \int_{-\frac{x}{\sqrt{3}}}^{\frac{x}{\sqrt{3}}}  
                      (x-\bar{x})^{2} dy                            \\
                  &=& \frac{1}{A} \frac{2}{\sqrt{3}} 
                      \int_{0}^{c_p} x (x-\bar{x})^{2}              \\
                  &=& \frac{1}{A} \frac{2}{\sqrt{3}} 
                      \int_{0}^{c_p}
                      ( x^{3}-2x^{2}\bar{x}+\bar{x}^{2}x ) dx           \\
                  &=& \frac{1}{A} \frac{2}{\sqrt{3}} 
                      \int_{0}^{c_p} ( x^{3}-\frac{4}{3}c_p x^{2}
                      + \frac{4}{9} c_p^{2} x ) dx                  \\
                  &=& \frac{1}{A} \frac{2}{\sqrt{3}} 
                      \left[ \frac{x^{4}}{4} - \frac{4}{9} c_p x^{3}
                      + \frac{2}{9} c_p^{2} x^{2}\right]_{0}^{c_p}      \\
                  &=& \frac{c_p^4}{A} \frac{2}{\sqrt{3}} 
                      \left[ \frac{1}{4}-\frac{4}{9}+\frac{2}{9} \right]  \\
                  &=& \frac{c_p^4}{A} \frac{2}{\sqrt{3}} 
                      \left[ \frac{1}{4}-\frac{2}{9} \right]  \\
                  &=& c_p^4 \frac{\sqrt{3}}{c_p^2} \frac{2}{\sqrt{3}} 
                           \frac{1}{36}  \\
                  &=& \frac{1}{18} c_p^{2} \\
  V_x = \sigma^2_x &=& \left( \frac{c_p}{3\sqrt{2}} \right)^2 \, ;
\end{eqnarray}
\begin{eqnarray}
  V_y = \sigma^2_y 
        &=& \frac{1}{A} \int_{0}^{c_p} dx
            \int_{-\frac{x}{\sqrt{3}}}^{\frac{x}{\sqrt{3}}}(y-\bar{y})^{2} dy \\
        &=& \frac{1}{A} \int_{0}^{c_p} \left[ \frac{y^{3}}{3} 
            \right]_{-\frac{x}{\sqrt{3}}}^{\frac{x}{\sqrt{3}}} dy            \\
        &=& \frac{1}{A} \frac{2}{3\sqrt{3}} 
            \int_{0}^{c_p} x^{3}dx \nonumber                        \\
        &=& \frac{1}{A} \frac{2}{9\sqrt{3}} 
            \left[ \frac{x^{4}}{4} \right]_{0}^{c_p}                \\
        &=& \frac{1}{A} \frac{2}{9\sqrt{3}} \frac{c_p^4}{4}      \\
        &=& \frac{\sqrt{3}}{c_p^2} \frac{2}{9\sqrt{3}} \frac{c_p^4}{4}  \\
        &=& \frac{1}{9} \frac{c_p^2}{2}  \\
        &=& \frac{1}{18} c_p^2  \\
  V_y = \sigma^2_y 
        &=& \left( \frac{c_p^{2}}{3\sqrt{2}} \right)^2 \, .
\end{eqnarray}
The covariance is given by:
\begin{eqnarray}
  V_{xy} &=& \frac{1}{A} \int \int (x-\bar{x}) (y-\bar{y}) dx dy         \\
        &=& \frac{1}{A} \int_{0}^{c_p} (x-\bar{x}) dx
            \int_{-\frac{x}{\sqrt{3}}}^{\frac{x}{\sqrt{3}}}(y-\bar{y}) dy     \\
        &=& \frac{1}{A} \int_{0}^{c_p} (x-\bar{x})
            \left[ 
              \frac{1}{2}y^2 - y \bar{y} 
            \right]_{-\frac{x}{\sqrt{3}}}^{\frac{x}{\sqrt{3}}}                \\
        &=& 0 \, .
\end{eqnarray}
Therefore: 
\begin{equation}
  \sigma_{x}=\sigma_{y}=\frac{c_p}{3\sqrt{2}} = 384.4 \mu{\rm m} \, .
\end{equation}
For the hexagonal case, the area of the overlapping region (shaded
zone in the right panel of figure \ref{Fig:SenseArea}) is givn by:
\begin{eqnarray}
  A & = & 6 \frac{1}{2} \frac{c_p}{\sqrt{3}} \frac{c_p}{2} \\
    & = & \frac{\sqrt{3}}{2}c_p^{2} \, .
\end{eqnarray}
By symmetry, $\bar{x} = \bar{y} = 0$.
The variance of the $x$ and $y$ coordinates are given by:
\begin{eqnarray}
  V_x = \sigma^2_x = \sigma^2_y =
        &=& \frac{1}{A} \int \int (x-\bar{x})^{2} dx dy \\
        &=& \frac{1}{A} \int \int x^{2} dx dy \\
        &=& \frac{2}{A}  \int_{-\frac{c_p}{2}}^{0}x^{2} dx 
            \int_{-\frac{x}{\sqrt{3}}-\frac{c_p}{\sqrt{3}}}
                ^{\frac{x}{\sqrt{3}}+\frac{c_p}{\sqrt{3}}} dy \nonumber \\
        &=& \frac{2}{A}\int_{-\frac{c_p}{2}}^{0}x^{2} 
            \left[ 2 \left( \frac{x}{\sqrt{3}}+\frac{c_p}{\sqrt{3}}  
            \right) \right] dx \\
        &=& \frac{2}{A}\frac{2}{\sqrt{3}} \int_{-\frac{c_p}{2}}^{0} 
            \left( x^{3}+ x^{2}c_p \right)dx \nonumber \\
        &=& \frac{2}{A}\frac{2}{\sqrt{3}} \left[ \frac{1}{4}
            x^4 +\frac{1}{3} x^3 c_p\right]_{-\frac{c_p}{2}}^{0} \\
        &=& \frac{2}{A}\frac{2}{\sqrt{3}} \left[ -\frac{1}{4}
            \frac{c_p^{4}}{16}+\frac{1}{3}\frac{c_p^{4}}{8}\right] \\
        &=& \frac{2}{A}\frac{2}{\sqrt{3}}
            \left[ \frac{1}{8} \left( \frac{1}{3}-\frac{1}{8} 
            \right) c_p^4 \right]\\
        &=& \frac{2}{A}\frac{2}{\sqrt{3}} \frac{1}{8} \frac{5}{24} c_p^4
         =  \frac{1}{A} \frac{5}{48\sqrt{3}} c_p^4 \\
        &=& \frac{2}{\sqrt{3}c_p^{2}} \frac{5}{48\sqrt{3}} c_p^4 
         =  \frac{2}{\sqrt{3}} \frac{5}{48\sqrt{3}} c_p^2 \\
        &=& \left( \sqrt{\frac{5}{2}}\frac{c_p}{6} \right)^2 \, .
\end{eqnarray}
As before, the covariance is given by:
\begin{eqnarray}
  V_{xy} &=& \frac{1}{A} \int \int (x-\bar{x}) (y-\bar{y}) dx dy         \\
        &=& \frac{2}{A}  \int_{-\frac{c_p}{2}}^{0} x dx 
            \int_{-\frac{x}{\sqrt{3}}-\frac{c_p}{\sqrt{3}}}
                ^{\frac{x}{\sqrt{3}}+\frac{c_p}{\sqrt{3}}} y dy \nonumber \\
        &=& \frac{2}{A}  \int_{-\frac{c_p}{2}}^{0} x dx 
            \left[
             \frac{1}{2} y^2
            \right]_{-\frac{x}{\sqrt{3}}-\frac{c_p}{\sqrt{3}}}
                   ^{\frac{x}{\sqrt{3}}+\frac{c_p}{\sqrt{3}}}   \nonumber \\
        &=& 0 \, .
\end{eqnarray}
Therefore:
\begin{equation}
  \sigma_{x}=\sigma_{y}=\sqrt{\frac{5}{2}}\frac{c_p}{6} = 429.8 \mu{\rm m} \, .
\end{equation}
